venom/props/venomExecPropsScript.sml
@@ -48,16 +48,16 @@ Theorem step_assert_behavior:
     eval_operand cond_op s = SOME cond ==>
     step_inst <| inst_id := id; inst_opcode := ASSERT;
                  inst_operands := [cond_op]; inst_outputs := [] |> s =
-    if cond = 0w then Revert (revert_state s) else OK s
+    if cond = 0w then Abort Revert_abort (revert_state s) else OK s
 Proof
   ACCEPT_TAC venomExecProofsTheory.step_assert_behavior
 QED
 
-(* REVERT instruction always produces Revert result *)
+(* REVERT instruction always produces Abort Revert_abort result *)
 Theorem step_revert_always_reverts:
   !inst s.
     inst.inst_opcode = REVERT ==>
-    step_inst inst s = Revert (revert_state s)
+    step_inst inst s = Abort Revert_abort (revert_state s)
 Proof
   ACCEPT_TAC venomExecProofsTheory.step_revert_always_reverts
 QED
